\documentclass{article}
\usepackage[utf8]{inputenc}
\usepackage{amsmath}
\usepackage{amsfonts}
\usepackage{cancel}
\usepackage{enumitem}
% \usepackage{txfonts}
\newcommand{\Z}{\mathbb{Z}}
\newcommand{\N}{\mathbb{N}}
\newcommand{\Q}{\mathbb{Q}}
\newcommand{\R}{\mathbb{R}}
\newcommand\litem[1]{\item{\bfseries#1\space}}

\title{kontrolloppgaver sinus forkurs}
\author{Martin Fosby}
\date{August 2018}

\begin{document}
\maketitle
\pagenumbering{gobble}

\paragraph{2}
\begin{enumerate}[label=\emph{\alph*})]
\litem{
  \begin{align*}
    \sqrt{12} - \sqrt{27} + \sqrt{48} &= \sqrt{4 * 3} - \sqrt{3 * 9} + \sqrt{12 * 4} \\ 
    &= 2 * \sqrt{3} - \sqrt{3} * 3 + \sqrt{3} * \sqrt{4} * 2 \\
    &= 2 * \sqrt{3} - \sqrt{3} * 3 + \sqrt{3} * 2 * 2 \\
    &= 2\sqrt{3} - 3\sqrt{3} + 4\sqrt{3} \\
    &= 3\sqrt{3}
  \end{align*}
  }
\litem{
  \begin{align*}
    \sqrt{18} - \sqrt{32} + \sqrt{2} &= \sqrt{9 * 2} - \sqrt{4 * 8} + \sqrt{2} \\
    &= 3\sqrt{2} - 2\sqrt{2 * 4} + \sqrt{2} \\
    &= 3\sqrt{2} - 2\sqrt{2} * 2 + \sqrt{2} \\
    &= 3\sqrt{2} - 4\sqrt{2} + \sqrt{2} \\
    &= 0 
  \end{align*}
  }
\litem{
\begin{align*}
    \sqrt{6} + \sqrt{54} - \sqrt{24} &= \sqrt{2 * 3} + \sqrt{9 * 6} - \sqrt{4 * 6} \\
    &= \sqrt{2 * 3} + 3\sqrt{2 * 3} - 2\sqrt{2 * 3} \\
    &= 2\sqrt{2 * 3} \\
    &= 2\sqrt{6}
\end{align*}
}
\end{enumerate}

\paragraph{1.196}
\begin{enumerate}[label=\emph{\alph*})]
\litem{
  \begin{align*}
    \sqrt{12} - \sqrt{27} + \sqrt{48} &= \sqrt{4 * 3} - \sqrt{3 * 9} + \sqrt{12 * 4} \\ 
    &= 2 * \sqrt{3} - \sqrt{3} * 3 + \sqrt{3} * \sqrt{4} * 2 \\
    &= 2 * \sqrt{3} - \sqrt{3} * 3 + \sqrt{3} * 2 * 2 \\
    &= 2\sqrt{3} - 3\sqrt{3} + 4\sqrt{3} \\
    &= 3\sqrt{3}
  \end{align*}
  }
\litem{
  \begin{align*}
    \sqrt{18} - \sqrt{32} + \sqrt{2} &= \sqrt{9 * 2} - \sqrt{4 * 8} + \sqrt{2} \\
    &= 3\sqrt{2} - 2\sqrt{2 * 4} + \sqrt{2} \\
    &= 3\sqrt{2} - 2\sqrt{2} * 2 + \sqrt{2} \\
    &= 3\sqrt{2} - 4\sqrt{2} + \sqrt{2} \\
    &= 0 
  \end{align*}
  }
\litem{
\begin{align*}
    \sqrt{6} + \sqrt{54} - \sqrt{24} &= \sqrt{2 * 3} + \sqrt{9 * 6} - \sqrt{4 * 6} \\
    &= \sqrt{2 * 3} + 3\sqrt{2 * 3} - 2\sqrt{2 * 3} \\
    &= 2\sqrt{2 * 3} \\
    &= 2\sqrt{6}
\end{align*}
}
\end{enumerate}

\end{document}